\documentclass{beamer}
\usepackage{amsmath,amssymb}
\usepackage{siunitx}
\sisetup{per-mode=symbol}
\usepackage{gvv}

\title{Matrix 5.5.32}
\author{ai25btech11015 -- M Sai Rithik}
\date{}

\begin{document}
\frame{\titlepage}

\begin{frame}
\frametitle{Problem}
If
\[
A = \myvec{1 & \cot x \\[4pt] -\cot x & 1},
\]
show that
\[
A^{\top} A^{-1} = 
\myvec{-\cos 2x & -\sin 2x \\[4pt] \sin 2x & -\cos 2x}.
\]
\end{frame}

\begin{frame}
\frametitle{Step 1: Determinant and Inverse}
\[
\det A = 1 + \cot^2 x = \csc^2 x.
\]
\[
A^{-1} 
= \frac{1}{\det A}\myvec{1 & -\cot x \\[4pt]\cot x & 1}
= \sin^2 x \,\myvec{1 & -\cot x \\[4pt]\cot x & 1}.
\]
\end{frame}

\begin{frame}
\frametitle{Step 2: Transpose and Product}
Transpose:
\[
A^{\top} = \myvec{1 & -\cot x \\[4pt]\cot x & 1}.
\]
Form the product:
\[
A^{\top} A^{-1} 
= \sin^2 x \;\myvec{1 & -t \\[4pt] t & 1}\;\myvec{1 & -t \\[4pt] t & 1}, 
\quad t=\cot x.
\]
\end{frame}

\begin{frame}
\frametitle{Step 3: Simplification}
Multiply matrices:
\[
\myvec{1 & -t \\[4pt] t & 1}\;\myvec{1 & -t \\[4pt] t & 1}
= \myvec{1-t^2 & -2t \\[4pt] 2t & 1-t^2}.
\]
Now substitute \(t=\frac{\cos x}{\sin x}\) and simplify:
\[
\sin^2 x(1-t^2) = -\cos 2x,
\quad 
\sin^2 x(-2t) = -\sin 2x,
\quad 
\sin^2 x(2t) = \sin 2x.
\]
\end{frame}

\begin{frame}
\frametitle{Final Result}
\[
A^{\top} A^{-1} =
\myvec{-\cos 2x & -\sin 2x \\[4pt] \sin 2x & -\cos 2x}.
\]
\end{frame}

\end{document}
