\documentclass[12pt]{article}
\usepackage[a4paper,margin=1in]{geometry}
\usepackage{amsmath,amssymb}
\usepackage{graphicx}
\usepackage{siunitx}
\sisetup{per-mode=symbol}
\usepackage{gvv}

\title{Matrix 5.5.32}
\author{ai25btech11015 -- M Sai Rithik}
\date{}

\begin{document}
\maketitle

\section*{Problem}
If
\begin{equation}
A=\myvec{1 & \cot x \\[4pt] -\cot x & 1 },
\end{equation}
show that
\begin{equation}
A^{\top}A^{-1}=\myvec{ -\cos2x & -\sin2x \\[4pt] \sin2x & -\cos2x }.
\end{equation}

\section*{Solution}

First compute the determinant of \(A\).
\begin{equation}
\det A = 1\cdot 1 - (\cot x)(-\cot x)
= 1 + \cot^2 x = \csc^2 x.
\end{equation}

Hence the inverse of \(A\) is
\begin{equation}
A^{-1} = \frac{1}{\det A}\myvec{1 & -\cot x \\[4pt] \cot x & 1}
= \sin^2 x \,\myvec{1 & -\cot x \\[4pt] \cot x & 1}.
\end{equation}

The transpose of \(A\) is
\begin{equation}
A^{\top}=\myvec{1 & -\cot x \\[4pt] \cot x & 1}.
\end{equation}

Form the product \(A^{\top}A^{-1}\). Using \(t=\cot x\) for brevity,
\begin{equation}
A^{\top}A^{-1}
= \sin^2 x \;\myvec{1 & -t \\[4pt] t & 1}\;\myvec{1 & -t \\[4pt] t & 1}.
\end{equation}

Compute the inside product:
\begin{equation}
\myvec{1 & -t \\[4pt] t & 1}\;\myvec{1 & -t \\[4pt] t & 1}
= \myvec{1-t^2 & -2t \\[4pt] 2t & 1-t^2 }.
\end{equation}

Now substitute \(t=\cot x=\dfrac{\cos x}{\sin x}\) and multiply by \(\sin^2 x\):
\begin{align}
\sin^2 x\,(1-t^2)
&= \sin^2 x\!\left(1-\frac{\cos^2 x}{\sin^2 x}\right)
= \sin^2 x\!\left(\frac{\sin^2 x-\cos^2 x}{\sin^2 x}\right)
= \sin^2 x - \cos^2 x
= -\cos 2x, \\
\sin^2 x\,(-2t)
&= -2\sin^2 x\cdot\frac{\cos x}{\sin x}
= -2\sin x\cos x
= -\sin 2x, \\
\sin^2 x\,(2t)
&= 2\sin^2 x\cdot\frac{\cos x}{\sin x}
= 2\sin x\cos x
= \sin 2x.
\end{align}

Therefore
\begin{equation}
A^{\top}A^{-1}
= \myvec{-\cos 2x & -\sin 2x \\[4pt] \sin 2x & -\cos 2x},
\end{equation}
as required.

\end{document}
